Replace definitions of order from AFP with ones from HOL for message justification other than wfp_on

Isabelle/CBCCasper.thy
@@ -1,6 +1,6 @@
 theory CBCCasper
 
-imports Main HOL.Real "Libraries/Strict_Order"
+imports Main HOL.Real "Libraries/Strict_Order" "Libraries/Restricted_Predicates"
 
 begin
 
@@ -336,15 +336,18 @@ type_synonym consensus_value_property = "consensus_value \<Rightarrow> bool"
 (* Message justification and lemmas *)
 (* ###################################################### *)
 
+definition (in Params) message_justification :: "message rel"
+  where 
+    "message_justification = {(m1, m2). {m1, m2} \<subseteq> M \<and> justified m1 m2}" 
+
 lemma (in Protocol) transitivity_of_justifications :
-  "transp_on justified M"
-  apply (simp add: transp_on_def)
-  by (meson Params.M_type Params.state_is_in_pow_M_i Protocol_axioms contra_subsetD justified_def)
+  "trans message_justification"
+  apply (simp add: trans_def message_justification_def justified_def)
+  by (meson Params.M_type Params.state_is_in_pow_M_i Protocol_axioms contra_subsetD)
 
 lemma (in Protocol) irreflexivity_of_justifications :
-  "irreflp_on justified M"
-  apply (simp add: irreflp_on_def)
-  apply (simp add: justified_def)
+  "irrefl message_justification"
+  apply (simp add: irrefl_def message_justification_def justified_def)
   apply (simp add: M_def)
   apply auto
 proof -
@@ -368,9 +371,18 @@ proof -
     using \<open>m \<in> justification m\<close> by blast
 qed
 
+lemma (in Protocol) message_cannot_justify_itself :
+  "(\<forall> m \<in> M. \<not> justified m m)"
+proof -
+  have "irrefl message_justification"
+    using irreflexivity_of_justifications by simp  
+  then show ?thesis
+    by (simp add: irreflexivity_of_justifications irrefl_def message_justification_def)
+qed
+
 lemma (in Protocol) justification_is_strict_partial_order_on_M :
-  "po_on justified M"
-  apply (simp add: po_on_def)
+  "strict_partial_order message_justification"
+  apply (simp add: strict_partial_order_def)
   by (simp add: irreflexivity_of_justifications transitivity_of_justifications)
 
 lemma (in Protocol) monotonicity_of_justifications :
@@ -380,11 +392,11 @@ lemma (in Protocol) monotonicity_of_justifications :
 
 lemma (in Protocol) strict_monotonicity_of_justifications :
   "\<forall> m m' \<sigma>. m \<in> M \<and> \<sigma> \<in> \<Sigma> \<and> justified m' m \<longrightarrow> justification m' \<subset> justification m"
-  by (metis M_type irreflexivity_of_justifications irreflp_on_def justified_def message_in_state_is_valid monotonicity_of_justifications psubsetI)
+  by (metis M_type message_cannot_justify_itself  justified_def message_in_state_is_valid monotonicity_of_justifications psubsetI)
 
 lemma (in Protocol) justification_implies_different_messages :
   "\<forall> m m'. m \<in> M \<and> m' \<in> M \<longrightarrow> justified m' m \<longrightarrow> m \<noteq> m'"
-  by (meson irreflexivity_of_justifications irreflp_on_def)
+  using message_cannot_justify_itself by auto
 
 lemma (in Protocol) only_valid_message_is_justified :
   "\<forall> m \<in> M. \<forall> m'. justified m' m \<longrightarrow> m' \<in> M"
@@ -424,6 +436,7 @@ lemma (in Protocol) monotonicity_of_card_of_justification :
   \<longrightarrow> card (justification m') < card (justification m)"
   by (meson M_type Protocol.strict_monotonicity_of_justifications Protocol_axioms justification_is_finite psubset_card_mono)
 
+(* TODO: Use Wellfounded.wf *)
 lemma (in Protocol) justification_is_well_founded_on_M :
   "wfp_on justified M"
 proof (rule ccontr) 
@@ -453,32 +466,5 @@ qed
 lemma (in Protocol) subset_of_M_have_minimal_of_justification :
   "\<forall> S \<subseteq> M. S \<noteq> \<emptyset> \<longrightarrow> (\<exists> m_min \<in> S. \<forall> m. justified m m_min \<longrightarrow> m \<notin> S)"
   by (metis justification_is_well_founded_on_M wfp_on_imp_has_min_elt wfp_on_mono)
-
-definition (in Params) state_transition :: "state rel"
-  where 
-    "state_transition = {(\<sigma>1, \<sigma>2). {\<sigma>1, \<sigma>2} \<subseteq> \<Sigma> \<and> is_future_state(\<sigma>1, \<sigma>2)}" 
-
-lemma (in Params) reflexivity_of_state_transition :
-  "refl_on \<Sigma> state_transition"  
-  apply (simp add: state_transition_def refl_on_def)
-  by auto
-
-lemma (in Params) transitivity_of_state_transition :
-  "trans state_transition"  
-  apply (simp add: state_transition_def trans_def)
-  by auto
-
-lemma (in Params) state_transition_is_preorder :
-  "preorder_on \<Sigma> state_transition"
-  by (simp add: preorder_on_def reflexivity_of_state_transition transitivity_of_state_transition)
-
-lemma (in Params) antisymmetry_of_state_transition :
-  "antisym state_transition"  
-  apply (simp add: state_transition_def antisym_def)
-  by auto
-
-lemma (in Params) state_transition_is_partial_order :
-  "partial_order_on \<Sigma> state_transition"
-  by (simp add: partial_order_on_def state_transition_is_preorder antisymmetry_of_state_transition)
 
 end
