Isabelle/Libraries/Strict_Order.thy
@@ -6,85 +6,84 @@
 
 theory Strict_Order
 
-imports Main Restricted_Predicates
+imports Main
 
 begin
 
 notation Set.empty ("\<emptyset>")
 
-(* Modified from: https://isabelle.in.tum.de/library/HOL/HOL/Order_Relation.html *)
-definition strict_linear_order_on :: "('a \<Rightarrow> 'a \<Rightarrow> bool) \<Rightarrow> 'a set \<Rightarrow> bool" 
+definition "strict_partial_order r \<equiv> trans r \<and> irrefl r"
+
+definition "strict_well_order_on A r \<equiv> strict_linear_order_on A r \<and> wf r"
+
+(* NOTE: In these definitions r is assumed to be strict partial order. *)
+definition upper_bound_on :: "'a set \<Rightarrow> 'a rel \<Rightarrow> 'a \<Rightarrow> bool"
   where 
-      "strict_linear_order_on P A \<equiv> po_on P A  \<and> total_on P A"
+    "upper_bound_on A r x = (\<forall> y. y \<in> A \<longrightarrow> (y, x) \<in> r \<or> x = y)"
 
-definition strict_well_order_on :: "('a \<Rightarrow> 'a \<Rightarrow> bool) \<Rightarrow> 'a set \<Rightarrow> bool" 
+definition maximum_on :: "'a set \<Rightarrow> 'a rel \<Rightarrow> 'a \<Rightarrow> bool"
   where 
-      "strict_well_order_on P A \<equiv> strict_linear_order_on P A  \<and> wfp_on P A"
+    "maximum_on A r x = (x \<in> A \<and> upper_bound_on A r x)" 
 
-definition upper_bound_on :: "('a \<Rightarrow> 'a \<Rightarrow> bool) \<Rightarrow> 'a set \<Rightarrow> 'a \<Rightarrow> bool"
+definition minimal_on :: "'a set \<Rightarrow> 'a rel \<Rightarrow> 'a \<Rightarrow> bool"
   where 
-    (* "upper_bound_on P A x = (\<forall> y \<in> A. P y x)" *)
-    "upper_bound_on P A x = (\<forall> y. y \<in> A \<longrightarrow> P y x)"
+    "minimal_on A r x = (x \<in> A \<and> (\<forall> y. (y, x) \<in> r \<longrightarrow> y \<notin> A))" 
 
-definition maximum_on :: "('a \<Rightarrow> 'a \<Rightarrow> bool) \<Rightarrow> 'a set \<Rightarrow> 'a \<Rightarrow> bool"
+definition maximal_on :: "'a set \<Rightarrow> 'a rel \<Rightarrow> 'a \<Rightarrow> bool"
   where 
-    "maximum_on P A x = (x \<in> A \<and> upper_bound_on P A x)" 
+    "maximal_on A r x = (x \<in> A \<and> (\<forall> y. (x, y) \<in> r \<longrightarrow> y \<notin> A))"
 
-definition minimal_on :: "('a \<Rightarrow> 'a \<Rightarrow> bool) \<Rightarrow> 'a set \<Rightarrow> 'a \<Rightarrow> bool"
-  where 
-    "minimal_on P A x = (x \<in> A \<and> (\<forall> y. P y x \<longrightarrow> y \<notin> A))" 
+lemma maximal_and_maximum_coincide_for_strict_linear_order :
+  "strict_linear_order_on A r \<Longrightarrow> maximal_on A r x = maximum_on A r x"
+  apply (simp add: strict_linear_order_on_def irrefl_def maximal_on_def maximum_on_def upper_bound_on_def total_on_def)
+  by (metis transE)
 
-definition maximal_on :: "('a \<Rightarrow> 'a \<Rightarrow> bool) \<Rightarrow> 'a set \<Rightarrow> 'a \<Rightarrow> bool"
-  where 
-    "maximal_on P A x = (x \<in> A \<and> (\<forall> y. P x y \<longrightarrow> y \<notin> A))"
-
-lemma "(\<not> A \<or> \<not> B) \<equiv> (A \<longrightarrow> \<not> B)"
-  by auto
-
-lemma "(A \<longrightarrow> \<not> B) \<equiv> (B \<longrightarrow> \<not> A)"
-  by linarith
-
-lemma "A = True \<longrightarrow> ((\<not> (A \<longrightarrow> B)) = (A \<longrightarrow> \<not> B))"
-  by auto
-
-lemma strict_partial_order_has_at_most_one_maximum :
-  "po_on P A
-  \<longrightarrow> {x. maximum_on P A x} \<noteq> \<emptyset> 
-  \<longrightarrow> is_singleton {x. maximum_on P A x}"
-proof (rule ccontr)
-  assume "\<not> (po_on P A \<longrightarrow> {x. maximum_on P A x} \<noteq> \<emptyset> \<longrightarrow> is_singleton {x. maximum_on P A x})"
-  then have "po_on P A \<longrightarrow> {x. maximum_on P A x} \<noteq> \<emptyset> \<longrightarrow> (\<exists> x1 x2. {x1, x2} \<subseteq> A \<and> x1 \<noteq> x2 \<and> (\<forall> y \<in> A. P y x1) \<and> (\<forall> y \<in> A. P y x2))"
-    apply (simp add: maximum_on_def upper_bound_on_def is_singleton_def)
-    apply auto
-    by blast
-  then show False
-    using po_on_imp_antisymp_on antisymp_on_def
-    (* The reason why \<open>...\<close> is required would be explored below. *)
-    by (metis \<open>\<not> (po_on P A \<longrightarrow> {x. maximum_on P A x} \<noteq> \<emptyset> \<longrightarrow> is_singleton {x. maximum_on P A x})\<close> insert_subset)
-qed
-
-lemma maximal_and_maximum_coincide_for_total_order :
-  "total_on P A \<Longrightarrow> maximal_on P A x = maximum_on P A x"
-  oops
-
-lemma "finite A \<longrightarrow> A \<noteq> \<emptyset> \<longrightarrow> (\<exists> x. maximal_on P A x) \<longrightarrow> (\<forall> x \<in> A. \<exists> y. y \<in> A \<and> P x y)"
-  apply (simp add:  maximal_on_def) 
-  oops
-
-lemma strict_partial_order_on_finite_set_has_maximal :
-  "po_on P A \<longrightarrow> finite A \<longrightarrow> A \<noteq> \<emptyset> \<longrightarrow> (\<exists> x. maximal_on P A x)"
+lemma strict_partial_order_on_finite_non_empty_set_has_maximal :
+  "strict_partial_order r \<longrightarrow> finite A \<longrightarrow> A \<noteq> \<emptyset> \<longrightarrow> (\<exists> x. maximal_on A r x)"
 proof (rule ccontr)
   (* NOTE: How to use \<not> for pure logic? #81 *)
-  assume "\<not> (po_on P A \<longrightarrow> finite A \<longrightarrow> A \<noteq> \<emptyset> \<longrightarrow> (\<exists> x. maximal_on P A x))"
-  have "finite A \<longrightarrow> A \<noteq> \<emptyset> \<longrightarrow> (\<exists> x. maximal_on P A x) \<longrightarrow> (\<forall> x \<in> A. \<exists> y. y \<in> A \<and> P x y)"
-    using maximal_on_def sorry 
-  show False
-    using po_on_def irreflp_on_def transp_on_def 
+  assume "\<not> (strict_partial_order r \<longrightarrow> finite A \<longrightarrow> A \<noteq> \<emptyset> \<longrightarrow> (\<exists> x. maximal_on A r x))"
+  moreover have "finite A \<longrightarrow> A \<noteq> \<emptyset> \<longrightarrow> (\<exists> x. maximal_on A r x) \<longrightarrow> (\<forall> x \<in> A. \<exists> y. (x, y) \<in> r \<longrightarrow> y \<in> A)"
+    using maximal_on_def by auto
+  ultimately show False
+    using strict_partial_order_def irrefl_def trans_def
     sorry
 qed
 
-lemma strict_linear_order_on_finite_set_has_one_maximum :
-  "strict_linear_order_on P A \<longrightarrow> finite A \<longrightarrow> A \<noteq> \<emptyset> \<longrightarrow> is_singleton {x. maximum_on P A x}"
+lemma strict_partial_order_has_at_most_one_maximum :
+  "strict_partial_order r
+  \<longrightarrow> {x. maximum_on A r x} \<noteq> \<emptyset> 
+  \<longrightarrow> is_singleton {x. maximum_on A r x}"
+proof (rule ccontr)
+  assume "\<not> (strict_partial_order r \<longrightarrow> {x. maximum_on A r x} \<noteq> \<emptyset> \<longrightarrow> is_singleton {x. maximum_on A r x})"
+  then have "strict_partial_order r \<longrightarrow> {x. maximum_on A r x} \<noteq> \<emptyset> \<longrightarrow> (\<exists> x1 x2. {x1, x2} \<subseteq> A \<and> x1 \<noteq> x2 \<and> (\<forall> y \<in> A. (y, x1) \<in> r) \<and> (\<forall> y \<in> A. (y, x2) \<in> r))"
+    apply (simp add: maximum_on_def upper_bound_on_def is_singleton_def strict_partial_order_def irrefl_def)
+    apply auto
+    (* sledgehammer *)
+  proof -
+    fix x :: 'a
+    assume a1: "\<forall>a. (a, a) \<notin> r"
+    assume a2: "trans r"
+    obtain aa :: "'a set \<Rightarrow> 'a" and aaa :: "'a set \<Rightarrow> 'a" where
+        f3: "aa (Collect (maximum_on A r)) \<in> Collect (maximum_on A r) \<and> aaa (Collect (maximum_on A r)) \<in> Collect (maximum_on A r) \<and> aa (Collect (maximum_on A r)) \<noteq> aaa (Collect (maximum_on A r))"
+      by (meson \<open>\<not> (strict_partial_order r \<longrightarrow> {x. maximum_on A r x} \<noteq> \<emptyset> \<longrightarrow> is_singleton {x. maximum_on A r x})\<close> is_singletonI')
+  have f4: "\<forall>A r a. maximum_on A r (a::'a) = (a \<in> A \<and> upper_bound_on A r a)"
+    using maximum_on_def by blast
+    then have f5: "(aaa (Collect (maximum_on A r)), aa (Collect (maximum_on A r))) \<in> r"
+      using f3 by (metis (no_types) CollectD upper_bound_on_def)
+    have "\<forall>a. a \<notin> A \<or> (a, aaa (Collect (maximum_on A r))) \<in> r \<or> aaa (Collect (maximum_on A r)) = a"
+      using f4 f3 by (metis CollectD upper_bound_on_def)
+  then show "\<exists>x1. x1 \<in> A \<and> (\<exists>x2. x2 \<in> A \<and> x1 \<noteq> x2 \<and> (\<forall>y\<in>A. (y, x1) \<in> r) \<and> (\<forall>y\<in>A. (y, x2) \<in> r))"
+    using f5 f4 f3 a2 a1 by (metis (no_types) CollectD transE)
+  qed
+  then show False
+    using strict_partial_order_def antisym_def
+    (* NOTE: Why \<open>...\<close> is required? *)
+    using \<open>\<not> (strict_partial_order r \<longrightarrow> {x. maximum_on A r x} \<noteq> \<emptyset> \<longrightarrow> is_singleton {x. maximum_on A r x})\<close> irrefl_def by fastforce
+qed
+
+lemma strict_linear_order_on_finite_non_empty_set_has_one_maximum :
+  "strict_linear_order_on A r \<longrightarrow> finite A \<longrightarrow> A \<noteq> \<emptyset> \<longrightarrow> is_singleton {x. maximum_on A r x}"
   oops
 
 end
